\documentclass{article}
\usepackage{graphicx} % Required for inserting images
\usepackage[margin=1.5cm]{geometry}
\title{Macroeconomics Homework 6}
\author{Alexandre Hsieh (ch132)}
\date{}

\begin{document}

\maketitle

\begin{enumerate}
    \item
        The statement is wrong. Ricardian Equivalence says that the household knows that the present discounted value of tax payments must be equal to the present discounted value of government spending (that is, $T_t$, $T_{t+1}$, and $B_t^G$ are irrelevant) so that \[C_t+\frac{C_t+1}{1+r_t}=Y_t-G_t+\frac{Y_{t+1}-G_{t+1}}{1+r_t}\] As shown above, $G_{t+1}$ is discounted by $1+r_t$, implying that the effect of $G_{t+1}$ is different from that of $G_t$. That is, a change in $G_t$ causes a larger effect on the equilibrium and the shift of the IS curve than $G_{t+1}$ does.
    \item 
    \begin{enumerate}
        \item \[U = \ln \left[ C_t - \frac{\theta_t}{2} N_t^2 \right]=\ln \left[ w_tN_t+D_t - \frac{\theta_t}{2} N_t^2
            \right]\]
            \[\frac{\partial U}{\partial N_t} = \frac{1}{ w_tN_t+D_t - \frac{\theta_t}{2} N_t^2} \cdot \left( w_t - \theta_t N_t \right) = 0\]
            Since the denominator must not be zero, $w_t-\theta_tN_t=0$. Then $w_t=\theta_tN_t$.
        \item
            \[D_t = A_t N_t - w_t N_t\]
            \[\frac{\partial D_t}{\partial N_t}=A_t-w_t=0\]
            \[w_t=A_t\]
        \item 
            Since $w_t=A_t$, we have $D_t=A_tN_t-A_tN_t=0$. This means that $D_t$ in equilibrium is zero, which   makes sense under perfect competition where firms cannot make an abnormal profit.
        \item
            \[C_t= w_tN_t+D_t= w_tN_t+A_tN_t-w_tN_t=A_tN_t=Y_t\]
        \item
            \[Y_t=A_tN_t=A_t\frac{w_t}{\theta_t}=\frac{A_t^2}{\theta_t}\]
            \[\frac{\partial Y_t}{\partial A_t} =\frac{2A_t}{\theta_t}>0\]
            \[\frac{\partial Y_t}{\partial \theta_t}=-\frac{A_t^2}{\theta_t^2}<0\]
        \item 
            \[U = \ln \left[ C_t - \frac{\theta_t}{1+\chi} N_t^{1+\chi} \right]=\ln \left[ w_tN_t+D_t -       \frac{\theta_t}{1+\chi} N_t^{1+\chi} \right]\]
            \[\frac{\partial U}{\partial N_t} = \frac{1}{w_tN_t+D_t - \frac{\theta_t}{1+\chi} N_t^{1+\chi}} \cdot \left(w_t -\theta_tN_t^{\chi} \right) = 0\]
            \[w_t =\theta_tN_t^{\chi}\]
            \[\frac{\partial D_t}{\partial N_t}=A_t-w_t=0\]
            \[w_t=A_t\]
            \[D_t=A_tN_t-A_tN_t=0\]
            \[C_t= w_tN_t+D_t= w_tN_t+A_tN_t-w_tN_t=A_tN_t=Y_t\]
            
            \[Y_t=A_tN_t=A_t \left(\frac{w_t}{\theta_t} \right)^{1/\chi}=A_t \left( \frac{A_t}{\theta_t} \right)^{1/\chi}=A_t^{\frac{\chi+1}{\chi}} \theta_t^{-\frac{1}{\chi}}\]
            \[\frac{\partial Y_t}{\partial A_t} = \left( \frac{\chi+1}{\chi} \right) A_t^{\frac{1}{\chi}} \theta_t^{-\frac{1}{\chi}}>0\]
            \[\frac{\partial Y_t}{\partial \theta_t} = -\frac{1}{\chi} \left( \frac{A_t}{\theta_t} \right)^{\frac{\chi+1}{\chi}}<0\]
    \end{enumerate}
    \item 
    \[V_t = D_t+\frac{D_{t+1}}{1+r_t}=Y_t+\frac{Y_{t+1}-(1+r_t+f_t)I_t}{1+r_t}=A_t K_t^\alpha + \frac{A_{t+1} I_t^\alpha - (1 + r_t + f_t) I_t}{1 + r_t}\]
    \[\frac{\partial V_t}{\partial I_t}=\frac{\alpha A_{t+1} I_t^{\alpha-1} - (1 + r_t + f_t)}{1 + r_t}=0\]
    \[\alpha A_{t+1} I_t^{\alpha-1} = 1 + r_t + f_t\]
    \[I_t=\left(\frac{1+r_t+f_t}{\alpha A_{t+1}}\right)^{1/{(\alpha-1)}}\]
    Since $0<\alpha<1$, $I_t$ is positively associated with $A_{t+1}$, while negatively associated with $r_t$ and $f_t$.
\end{enumerate}

\end{document}
