\documentclass{article}
\usepackage{graphicx} % Required for inserting images
\usepackage[margin=1.5cm]{geometry}
\usepackage{amsmath}

\title{ECON 502}
\author{Alexandre Hsieh}
\date{Homework 4 Part 3}

\begin{document}

\maketitle

\section{A}
\begin{enumerate}
    \item %1
    \begin{itemize}
        \item[i)] 
            $\int_{0}^{1} \int_{0}^{1} k(1 - xy) \,dy\,dx = 1$
            \newline $\int_{0}^{1} \left[ k \left( y - x\frac{y^2}{2} \right) \right]_{y=0}^{y=1} \,dx=\int_{0}^{1} k \left( 1 - \frac{x}{2} \right) \,dx=\left[ k \left( x - \frac{x^2}{4} \right) \right]_{x=0}^{x=1}=k \left(\frac{3}{4} \right)=1$
            \newline $k=\frac{4}{3}$
        \item[ii)] 
            $f_X(x) = \int_{0}^{1} \frac{4}{3}(1-xy) \,dy =\frac{4}{3} \left[y-\frac{xy^2}{2} \right]_{y=0}^{y=1} = \frac{4}{3}-\frac{2}{3}x$ 
            \newline $E(X)=\int_{0}^{1} x \left( \frac{4}{3}-\frac{2}{3}x\right)\ dx
            =\int_{0}^{1} \left( \frac{4}{3}x-\frac{2}{3}x^2\right)\ dx
            =\left[ \frac{2}{3}x^2 - \frac{2}{9}x^3 \right]_{0}^{1}=\frac{4}{9}$
            \newline $V(X)=E(X^2)-[E(X)]^2
            =\int_{0}^{1} x^2 \left( \frac{4}{3}-\frac{2}{3}x\right)\ dx-\frac{16}{81}
            =\left[ \frac{4}{9}x^3 - \frac{1}{6}x^4 \right]_{0}^{1}-\frac{16}{81}=\frac{13}{162}$
        \item[iii)] 
            $f_Y(y) = \int_{0}^{1} \frac{4}{3}(1-xy) \,dx =\frac{4}{3} \left[x-\frac{x^2y}{2} \right]_{x=0}^{x=1} = \frac{4}{3}-\frac{2}{3}y$ 
            \newline $E(Y)=\int_{0}^{1} y \left( \frac{4}{3}-\frac{2}{3}y\right)\ dy
            =\int_{0}^{1} \left( \frac{4}{3}y-\frac{2}{3}y^2\right)\ dy
            =\left[ \frac{2}{3}y^2 - \frac{2}{9}y^3 \right]_{0}^{1}=\frac{4}{9}$
            \newline $V(Y)=E(Y^2)-[E(Y)]^2
            =\int_{0}^{1} y^2 \left( \frac{4}{3}-\frac{2}{3}y\right)\ dy-\frac{16}{81}
            =\left[ \frac{4}{9}y^3 - \frac{1}{6}y^4 \right]_{0}^{1}-\frac{16}{81}=\frac{13}{162}$
        \item[iv)] $E(X+Y) = E(X) + E(Y)=\frac{4}{9}+\frac{4}{9}=\frac{8}{9}$
    \end{itemize}
    \item %2
    \begin{itemize}
        \item[i)] 
            $\int_{0}^{1} \int_{0}^{1} (cx+y) \,dy\,dx = 1$
            \newline $\int_{0}^{1} \int_{0}^{1} (cx+y) \,dy\,dx
            =\int_{0}^{1} \left[ (cxy+\frac{y^2}{2})\right]_{0}^{1}\,dx
            =\int_{0}^{1} (cx+\frac{1}{2})\,dx
            =\left[ (\frac{cx^2}{2}+\frac{x}{2})\right]_{0}^{1}=\frac{c+1}{2}=1$
            \newline $c=1$
        \item[ii)]
        $f_X(x) = \int_{0}^{1} (x+y) \,dy =\left[xy+\frac{y^2}{2} \right]_{y=0}^{y=1} = x+\frac{1}{2}$ 
            \newline $E(X)=\int_{0}^{1} x (x+\frac{1}{2}) dx
            =\int_{0}^{1} (x^2+\frac{1}{2}x)\ dx
            =\left[ \frac{x^3}{3} + \frac{x^2}{4} \right]_{0}^{1}=\frac{7}{12}$
            \newline $V(X)=E(X^2)-[E(X)]^2
            =\int_{0}^{1} x^2 (x+\frac{1}{2}) dx-\frac{49}{144}
            =\left[ \frac{x^4}{4} + \frac{x^3}{6} \right]_{0}^{1}-\frac{49}{144}=\frac{11}{144}$
        \item[iii)] 
         $f_Y(y) = \int_{0}^{1} (x+y) \,dx =\left[xy+\frac{x^2}{2} \right]_{x=0}^{x=1} = y+\frac{1}{2}$ 
            \newline $E(Y)=\int_{0}^{1} y (y+\frac{1}{2}) dy
            =\int_{0}^{1} (y^2+\frac{1}{2}y)\ dy
            =\left[ \frac{y^3}{3} + \frac{y^2}{4} \right]_{0}^{1}=\frac{7}{12}$
            \newline $V(Y)=E(Y^2)-[E(Y)]^2
            =\int_{0}^{1} y^2 (y+\frac{1}{2}) dy-\frac{49}{144}
            =\left[ \frac{y^4}{4} + \frac{y^3}{6} \right]_{0}^{1}-\frac{49}{144}=\frac{11}{144}$
        \item[iv)]
        $P(0.2\leq X\leq 0.6, \space 0.2\leq Y\leq 0.6)=\int_{0.2}^{0.6}\int_{0.2}^{0.6} (x + y) \,dy \,dx=\int_{0.2}^{0.6} \left[ xy + \frac{y^2}{2} \right]_{0.2}^{0.6} \,dx=\int_{0.2}^{0.6}(0.4x+0.16)\ dx=\left[ 0.2x^2+0.16x\right]_{0.2}^{0.6}=0.128$
    \end{itemize} 
    \item %3
    \begin{itemize}
        \item[i)] 
        $h(x|y)=\frac{f(x,y)}{f_Y(y)}=\frac{2}{\int_{0}^{y} 2 \, dx}=\frac{1}{y}$
        \newline $h(x|0.5)=h(0.5|0.5)=\frac{1}{0.5}=2$
        \item[ii)] 
        $g(y|x)=\frac{f(x,y)}{f_X(x)}=\frac{2}{\int_{x}^{1} 2 \, dy}=\frac{1}{1-x}$
        \newline $g(y|0.5)=g(0.5|0.5)=\frac{1}{1-0.5}=2$
        \item[iii)] $P(Y>0.5|X=0.5) = \int_{0.5}^{1} g(y|0.5) \, dy=\int_{0.5}^{1}2\, dy=1$
        \item[iv)]
        $E(Y|X=x)=\int_{x}^{1}y\cdot g(y|x)\, dy=\frac{1}{1-x}\left[\frac{y^2}{2}\right]_{y=x}^{y=1}=\frac{1+x}{2}$
        \newline $VAR(Y|X=x)=E(Y^2|X=x)-[E(Y|X=x)]^2=\int_{x}^{1}y^2\cdot g(y|x)\, dy-\frac{(1+x)^2}{4}
        =\frac{1}{1-x}\left[\frac{y^3}{3}\right]_{y=x}^{y=1}-\frac{(1+x)^2}{4}=\frac{(1-x)^2}{12}$
        \item[v)]
        $E(X|Y=y)=\int_{0}^{y}x\cdot h(x|y)\, dx=\frac{1}{y}\left[\frac{x^2}{2}\right]_{x=0}^{x=y}=\frac{y}{2}$
        \newline $VAR(X|Y=y)=E(X^2|Y=y)-[E(X|Y=y)]^2=\int_{0}^{y}x^2\cdot h(x|y)\, dx-\frac{y^2}{4}
        =\frac{1}{y}\left[\frac{x^3}{3}\right]_{x=0}^{x=y}-\frac{y^2}{4}=\frac{y^2}{12}$
        \item[vi)]
        $COV(X,Y)=E(XY)-E(X)E(Y)=\int_{0}^{1}\int_{x}^{1} xy\cdot 2\, dy\, dx-\int_{0}^{1}x\cdot 2\, dy-\int_{0}^{1} y\cdot 2\, dx=\frac{1}{4}-\frac{1}{3}\cdot \frac{2}{3}=\frac{1}{36}$
    \end{itemize}
    \item %4 
    UIN = 665092599 such that $E(X)=9$ and $E(Y)=9$
    \begin{itemize}
        \item[i)] $Y \sim N(E(Y), VAR(Y))=Y\sim N(9,5)$
        \item[ii)]
        $E(Y|X=3)=E(Y)+\frac{COV(X,Y)}{VAR(X)}(X-E(X))=9+\frac{5}{10}(3-9)=6$
        \newline $Var(Y|X=3)=VAR(Y)-\frac{COV(X,Y)^2}{VAR(X)}=\frac{5}{2}$
        \newline $(Y|X=3)\sim N(6,\frac{5}{2})$
        \newline $E(X|Y=-2)=E(X)+\frac{COV(X,Y)}{VAR(Y)}(Y-E(Y))=9+\frac{5}{5}(-2-9)=-2$
        \newline $Var(X|Y=-2)=VAR(X)-\frac{COV(X,Y)^2}{VAR(Y)}=5)$
        \newline $(X|Y=-2)\sim N(-2,5)$
    \end{itemize}
    \item %5
    $E(Y) = E(E(Y|\lambda)]=E(\lambda)=\alpha\beta$
    \newline $V(Y) = E(E(Y^2|\lambda)]-\{E(E(Y|\lambda)]\}^2=E(\lambda)+E(\lambda^2)-\alpha^2\beta^2
    =\alpha\beta+\{VAR(\lambda)+[E(\lambda)]^2\}-\alpha^2\beta^2
    =\alpha\beta+\{VAR(\lambda)+[E(\lambda)]^2\}-\alpha^2\beta^2
    =\alpha\beta+\alpha\beta^2+\alpha^2\beta^2-\alpha^2\beta^2=\alpha\beta(1+\beta)$
    \item %6
    For $0\le y\le 1$:\space $F_Y(y) =\int_{0}^{y}tdt =\left[\frac{t^2}{2}\right]_0^y=\frac{y^2}{2}$
    \newline For $1 < y \le 1.5$:\space$F_Y(y)=\int_{0}^{1}tdt+\int_{1}^{y}1dt=\frac{1}{2}+[t]_1^y=y-\frac{1}{2}$
    \newline Therefore, the CDF of $Y$ is:
    \[F_Y(y) =
    \begin{cases}
    0, & \text{} y < 0 \\
    \frac{y^2}{2},  & \text{} 0 \le y \le 1 \\
    y - \frac{1}{2}, & \text{} 1 < y \le 1.5 \\
    1, & \text{} y > 1.5
    \end{cases}\]
    \newline Since $U=10Y-4$, $Y=\frac{U+4}{10}$. Then the CDF of $U$ is:
    \[F_U(u) =
    \begin{cases}
    0, &\text{} u < -4 \\
    \frac{(u+4)^2}{200}, &\text{} -4 \le u \le 6 \\
    \frac{u - 1}{10}, &\text{} 6 < u \le 11 \\
    1, &\text{} u > 11
    \end{cases}\]
    $f_U(u) = \frac{d}{du} F_U(u)$, then:
    \[f_U(u) =
    \begin{cases}
    \frac{u+4}{100}, &\text -4 \le u \le 6 \\
    \frac{1}{10}, &\text 6 < u \le 11 \\
    0, &\text{elsewhere}
    \end{cases}\]
    \item %7    
    \begin{itemize}
        \item[i)] Since $U=Y^m$, $Y=U^{1/m}$. The Jacobian says $\left|\frac{dY}{dU}\right|=\left|\frac{1}{dU}U^{1/m}\right|=\frac{1}{m}U^{\frac{1-m}{m}}$. Then:
        \[f_U(u) = f_Y(g^{-1}(u)) \left| \frac{dY}{dU} \right|=\left( \frac{m}{\alpha}U^{\frac{m-1}{m}}e^{-\frac{U}{\alpha}}\right)\cdot\left(\frac{1}{m}U^{\frac{1-m}{m}}\right)=\frac{1}{\alpha}e^{-\frac{u}{\alpha}}\]
        \item[ii)]
        $E(Y^k)=\int_{0}^{\infty} y^k\left( \frac{m}{\alpha}y^{m-1}e^{-\frac{y^m}{\alpha}}\right)dy
        =\left( \frac{m}{\alpha} \cdot \frac{1}{m} \right) \alpha^{\frac{k+m-1}{m}} \alpha^{\frac{1}{m}} \int_{0}^{\infty} t^{\frac{k+m-1}{m}} t^{\frac{1}{m} - 1} e^{-t} dt
        =\alpha^{k/m} \int_{0}^{\infty} t^{k/m} e^{-t} dt
        \newline =\alpha^{k/m} \Gamma\left(\frac{k}{m} + 1\right)$
    \end{itemize}
    \item %8
    \begin{itemize}
        \item[i)] 
        $M_{Y_i}(t) = E[e^{tY_i}] = e^{\lambda_i(e^t - 1)}$. Let $\Theta = \sum_{i=1}^{n} Y_i$, then: $M_\Theta(t) = M_{Y_1}(t) M_{Y_2}(t) \cdots M_{Y_n}(t)$ such that $M_\Theta(t) = e^{\left( \sum_{i=1}^{n} \lambda_i \right) (e^t - 1)}$. 
        \newline Then let $\lambda = \sum_{i=1}^{n} \lambda_i$ such that $M_\Theta(t) = e^{\lambda (e^t - 1)}$. The probability function is \[P(\sum_{i=1}^{n}Y_i=\theta) = \frac{e^{-\lambda} \lambda\theta}{\theta!}, \quad\theta= 0,1,2,\ldots,\quad\lambda =\sum_{i=1}^{n}\lambda_i\].
        \item[ii)] 
        $P(Y_1=\theta|\sum_{i=1}^{n}Y_i=m)=\frac{\left( \frac{e^{-\lambda_1}\lambda_1^\theta}{\theta!}\right) \left(\frac{e^{-\lambda'}(\lambda')^{m-\theta}}{(m-\theta)!}\right)}{\frac{e^{-\lambda} \lambda\theta}{\theta!}},\space\lambda =\sum_{i=1}^{n}\lambda_i,\space\lambda'=\lambda-\lambda_1$. Then we can find that it is a binomial distribution:
        \[P(Y_1=\theta\mid\sum_{i=1}^{n}Y_i=m)=\binom{m}{\theta} p^\theta (1-p)^{m-\theta}, \quad \theta = 0, 1, \ldots, m\]
        \item[iii)]
        $P(Y_1 + Y_2 = \theta \mid \sum_{i=1}^{n} Y_i = m) = \binom{m}{\theta}(\frac{p_1+p_2}{2})^\theta (1-\frac{p_1+p_2}{2})^{m-\theta}, \quad \theta = 0, 1, \ldots, m$
    \end{itemize}
\end{enumerate}

\section{B}
\begin{enumerate}
    \item No.140
    \begin{itemize}
        \item[a)] Since the moment generating function of the Gamma distribution is $(1-\beta t)^{-\alpha}$, $M(t) = (1 - 4t)^{-2}$ forms a Gamma distribution of $Gamma(2,4)$.
        \item[b)] Since the moment generating function of the exponential distribution is $\frac{1}{1-\theta t}$, $M(t)=\frac{1}{1-3.2 t}$ forms an exponential distribution of $Exp(3.2)$.
        \item[c)] Since the moment generating function of the normal distribution is $e^{\mu t+\frac{1}{2}\sigma^2t^2}$, $M(t)=e^{-5t+6t^2}$ forms a normal distribution of $Norm(-5,12)$.
    \end{itemize}
    \item No.144
    \begin{itemize}
        \item[a)] $\int_{-\infty}^{\infty} k e^{-y^2/2} dy = 1$. Then $k\sqrt{2\pi} = 1\implies k=\frac{1}{\sqrt{2\pi}}$.
        \item[b)] $M_Y(t) = E(e^{tY}) = \int_{-\infty}^{\infty}e^{ty}\frac{1}{\sqrt{2\pi}}e^{-y^2/2}\,dy
        =e^{t^2/2}\left(\frac{1}{\sqrt{2\pi}}\int_{-\infty}^{\infty}e^{-\frac{(y-t)^2}{2}}dy\right)=e^{t^2/2}$
        \item[c)] $E(Y)=M_Y'(0)=te^{t^2/2}|_{t=0}=0$
        \newline $V(Y)=E(Y^2)-(E(Y))^2=M_Y''(0)=(1+t^2)e^{t^2/2}|_{t=0}-0=1$
    \end{itemize}
    \item No.146
    \newline Based on Chebyshev's inequality, $P(|Y-\mu|<k\sigma)\ge1-\frac{1}{k^2}$. To find an interval with probability greater than $1-0.1=0.9$, let $\frac{1}{k^2}=0.1 \implies k=\sqrt{10}$. Then $P(|Y-\mu|<k\sigma)=P(-k\sigma+\mu<Y<k\sigma+\mu)\approx P(12352<Y<37648)$. The suggested mileage interval is $(12352 \text{ miles}, 37648 \text{ miles})$.
    \item No.187
     \begin{itemize}
        \item[a)] Let $m=2$ and $\alpha=10$ such that $f(y) = \frac{2y^{2-1}}{10}e^{-y^2 / 10} = \frac{y}{5}e^{-y^2 / 10}, \quad y \ge 0$. $P(Y > 5)=\int_{5}^{\infty} \frac{1}{5} y e^{-y^2 / 10} dy=$
        \newline Let $u = \frac{y^2}{10}$. Then $du = \frac{2y}{10} dy\implies \frac{1}{5} y dy = du$. Then $P(Y>5)=\int_{2.5}^{\infty}e^{-u}du=e^{-2.5}\approx 0.08$
        \item[b)] Let $p=P(Y\le5)=1-P(Y > 5)=1-e^{-2.5}=0.92$, then $P(X=1)=\binom{3}{1}p^1(1-p)^{3-1}
        =3\cdot0.92\cdot(0.08)^2\approx 0.02$
    \end{itemize}
\end{enumerate}
\end{document}
